bedrock2/src/bedrock2Examples/LiveVerif/examples/min.v
@@ -20,4 +20,44 @@ Derive u_min SuchThat (fun_correct! u_min) As u_min_ok.                         
 }                                                                          /**.
 Defined.
 
+Lemma nth_function_correct: forall fs n specs spec default,
+    List.nth n specs default = spec ->
+    functions_correct fs specs ->
+    spec fs.
+Proof.
+  unfold functions_correct. intros.
+  Search List.Forall List.nth.
+Admitted.
+
+Definition minl: list Z -> Z := List.fold_right Z.min 0.
+
+#[export] Instance spec_of_u_min3: fnspec :=                                    .**/
+
+uintptr_t u_min3 (uintptr_t a, uintptr_t b, uintptr_t c) /**#
+  ghost_args := (R: mem -> Prop);
+  requires t m := R m;
+  ensures t' m' retv := t' = t /\ R m' /\
+      \[retv] = minl [| \[a]; \[b]; \[c] |] #**/                           /**.
+Derive u_min3 SuchThat (fun_correct! u_min3) As u_min3_ok.                      .**/
+{                                                                          /**.
+(*   uintptr_t r = u_min(a, b); *)
+  eapply wp_call.
+  { ltac1:(
+    let fname := constr:("u_min") in
+    let s := lazymatch constr:(_ : ProgramLogic.spec_of fname) with ?sp => sp end in
+    let s' := eval unfold s in s in
+    let new_callee_list := open_constr:(cons s _) in
+    lazymatch goal with
+    | H: functions_correct ?fs ?l |- _ =>
+        let callee_list_evar := strip_conss l in
+        unify callee_list_evar new_callee_list
+    end;
+
+    idtac s).
+    eapply (nth_function_correct _ O) in H. 2: cbn [List.nth]; reflexivity.
+    unfold spec_of_u_min in H.
+    eapply H.
+  }
+Abort.
+
 End LiveVerif. Comments .**/ //.
