bedrock2/src/bedrock2Examples/LiveVerif/LiveSnippet.v
@@ -3,6 +3,8 @@ Require Import bedrock2.Syntax.
 
 Inductive snippet :=
 | SAssign(is_decl: bool)(x: string)(e: Syntax.expr)
+| SCall(lhs: option (bool (* is_decl *) * string (* varname *)))
+       (fname: string)(args: list Syntax.expr)
 | SStore(sz: access_size)(addr val: Syntax.expr)
 | SIf(cond: Syntax.expr)
 | SElse
