bedrock2/src/bedrock2Examples/LiveVerif/LiveVerifLib.v
@@ -20,6 +20,7 @@ Require Export bedrock2.WordNotations.
 Require Export bedrock2.find_hyp.
 Require Export bedrock2.HeapletwiseHyps.
 Require Export bedrock2.bottom_up_simpl_ltac1.
+Require Export bedrock2.TacticError.
 Require Export bedrock2Examples.LiveVerif.LiveRules.
 Require Export bedrock2Examples.LiveVerif.PackageContext.
 Require Export bedrock2Examples.LiveVerif.LiveProgramLogic.
